test/StandardLibrary/Collections.dfy
@@ -1,15 +1,46 @@
 include "../../src/StandardLibrary/UInt.dfy"
 include "../../src/StandardLibrary/StandardLibrary.dfy"
-include "../../src/StandardLibrary/IO.dfy"
+include "../../src/StandardLibrary/Collections.dfy"
 
 module TestIO {
   import opened StandardLibrary
   import opened UInt = StandardLibrary.UInt
-  import opened IO
+  import opened Collections
 
   method {:test} IntSeqEnumerator() {
+    var testSeq := [1, 2, 3];
+    var seqEnum := new SeqEnumerator<int>(testSeq);
+      
+    var res := seqEnum.Next();
+    expect res.Success? && res.value.Some? && res.value.get == 1;
+    res := seqEnum.Next();
+    expect res.Success? && res.value.Some? && res.value.get == 2;
+    res := seqEnum.Next();
+    expect res.Success? && res.value.Some? && res.value.get == 3;
+    res := seqEnum.Next();
+    expect res.Success? && res.value == None();
+    res := seqEnum.Next();
+    expect res.Failure?;
+  }
+
+  method {:test} IntSeqAggregator() {
+    var seqAgg := new SeqAggregator<int>();
+
+    var res2 := seqAgg.Accept(1);
+    expect res2.Success? && res2.value && seqAgg.s == [1];
+    res2 := seqAgg.Accept(2);
+    expect res2.Success? && res2.value && seqAgg.s == [1, 2];
+    res2 := seqAgg.End();
+    expect res2.Success? && res2.value;
+    res2 := seqAgg.Accept(1);
+    expect res2.Failure?;
+    res2 := seqAgg.End();
+    expect res2.Failure?;
+  }
+  
+  method {:test} IntSeqChunkEnumerator() {
     var testSeq := [1, 2, 3, 4, 5];
-    var seqEnum := new SeqEnumerator<int>(testSeq, 2);
+    var seqEnum := new SeqChunkEnumerator<int>(testSeq, 2);
       
     var res := seqEnum.Next();
     expect res.Success? && res.value.Some? && res.value.get == [1, 2];
@@ -23,8 +54,8 @@ module TestIO {
     expect res.Failure?;
   }
 
-  method {:test} IntSeqAggregator() {
-    var seqAgg := new SeqAggregator<int>();
+  method {:test} IntSeqChunkAggregator() {
+    var seqAgg := new SeqChunkAggregator<int>();
 
     var res2 := seqAgg.Accept([1,2,3]);
     expect res2.Success? && res2.value && seqAgg.s == [1,2,3];
